ROOT
@@ -1,0 +1,8 @@
+session Set_Proc = HOL +
+  sessions
+    "HOL-Library"
+    Graph_Theory
+    ZFC_in_HOL
+  theories
+    Logic
+    Set_Proc
